CoqOfRust/move_sui/proofs/move_bytecode_verifier/type_safety.v
@@ -61,7 +61,7 @@ Ltac unfold_state_monad :=
     "return!toS!", "liftS!", "readS!";
   cbn.
 
-Ltac destruct_push :=
+Ltac destruct_abstract_push :=
   unfold TypeSafetyChecker.Impl_TypeSafetyChecker.push;
   with_strategy opaque [AbstractStack.push] unfold_state_monad;
   match goal with
@@ -72,78 +72,92 @@ Ltac destruct_push :=
   end;
   destruct AbstractStack.push as [[[[]|] ?stack_ty]|]; cbn; [|exact I | exact I].
 
+Ltac destruct_abstract_pop H_interpreter :=
+  unfold_state_monad;
+    let H_pop := fresh "H_pop" in
+    match goal with
+    | |- context[AbstractStack.pop ?stack] =>
+      pose proof (
+        AbstractStack.flatten_pop stack
+      ) as H_pop
+    end;
+    destruct AbstractStack.pop as [[[?operand_ty |] ?stack_ty] |];
+      cbn; [|exact I | exact I];
+    rewrite H_pop in H_interpreter; cbn in H_interpreter;
+    clear H_pop.
+
 Lemma progress
     (ty_args : list _Type.t) (function : loader.Function.t) (resolver : loader.Resolver.t)
     (instruction : Bytecode.t)
     (pc : Z) (locals : Locals.t) (interpreter : Interpreter.t)
     (type_safety_checker : TypeSafetyChecker.t)
     (H_interpreter : IsInterpreterContextOfType.t locals interpreter type_safety_checker) :
+  let state := {|
+    State.pc := pc;
+    State.locals := locals;
+    State.interpreter := interpreter;
+  |} in
   match
     verify_instr instruction pc type_safety_checker,
-    execute_instruction ty_args function resolver instruction (pc, locals, interpreter)
+    execute_instruction ty_args function resolver instruction state
   with
   | Panic.Value (Result.Ok _, type_safety_checker'),
-    Panic.Value (Result.Ok _, (_, locals', interpreter')) =>
+    Panic.Value (Result.Ok _, state') =>
+    let '{|
+      State.pc := _;
+      State.locals := locals';
+      State.interpreter := interpreter';
+    |} := state' in
     IsInterpreterContextOfType.t locals' interpreter' type_safety_checker'
   | _, _ => True
   end.
 Proof.
-  destruct instruction eqn:H_instruction_eq; cbn;
+  Opaque AbstractStack.flatten.
+  destruct interpreter as [[stack]].
+  destruct instruction eqn:H_instruction_eq; cbn in *;
     unfold IsInterpreterContextOfType.t, IsStackValueOfType.t in H_interpreter.
   { guard_instruction Bytecode.Pop.
-    unfold_state_monad.
-    pose proof (AbstractStack.flatten_pop type_safety_checker.(TypeSafetyChecker.stack)) as H_pop.
-    destruct AbstractStack.pop as [[operand stack'] |]; cbn; [|exact I].
-    destruct operand as [operand|]; cbn; [|exact I].
-    rewrite H_pop in H_interpreter.
+    destruct_abstract_pop H_interpreter.
     admit.
   }
   { guard_instruction Bytecode.Ret.
     admit.
   }
   { guard_instruction (Bytecode.BrTrue z).
-    unfold_state_monad.
-    pose proof (AbstractStack.flatten_pop type_safety_checker.(TypeSafetyChecker.stack)) as H_pop.
-    destruct AbstractStack.pop as [[operand_ty stack'] |]; cbn; [|exact I].
-    destruct operand_ty as [operand_ty|]; cbn; [|exact I].
-    rewrite H_pop in H_interpreter; clear H_pop.
+    destruct_abstract_pop H_interpreter.
     pose proof SignatureToken.t_beq_is_valid operand_ty SignatureToken.Bool as H_beq.
     destruct SignatureToken.t_beq; cbn; [|exact I].
     replace operand_ty with SignatureToken.Bool in H_interpreter by sfirstorder; clear H_beq.
     unfold Stack.Impl_Stack.pop_as, Stack.Impl_Stack.pop; cbn.
     unfold_state_monad.
-    destruct interpreter, operand_stack; cbn in *.
-    inversion_clear H_interpreter as [|operand ? stack ? H_operand_bool H_stack]; cbn.
+    cbn in *.
+    inversion_clear H_interpreter as [|operand ? stack' ? H_operand_bool H_stack']; cbn.
     assert (exists b, operand = ValueImpl.Bool b) as [b H_operand_eq]. {
       destruct operand; cbn; try contradiction; sfirstorder.
     }
     rewrite H_operand_eq; clear H_operand_eq; cbn.
-    apply H_stack.
+    apply H_stack'.
   }
   { guard_instruction (Bytecode.BrFalse z).
-    unfold_state_monad.
-    pose proof (AbstractStack.flatten_pop type_safety_checker.(TypeSafetyChecker.stack)) as H_pop.
-    destruct AbstractStack.pop as [[operand_ty stack'] |]; cbn; [|exact I].
-    destruct operand_ty as [operand_ty|]; cbn; [|exact I].
-    rewrite H_pop in H_interpreter; clear H_pop.
+    destruct_abstract_pop H_interpreter.
     pose proof SignatureToken.t_beq_is_valid operand_ty SignatureToken.Bool as H_beq.
     destruct SignatureToken.t_beq; cbn; [|exact I].
     replace operand_ty with SignatureToken.Bool in H_interpreter by sfirstorder; clear H_beq.
     unfold Stack.Impl_Stack.pop_as, Stack.Impl_Stack.pop; cbn.
     unfold_state_monad.
-    destruct interpreter, operand_stack; cbn in *.
-    inversion_clear H_interpreter as [|operand ? stack ? H_operand_bool H_stack]; cbn.
+    cbn in *.
+    inversion_clear H_interpreter as [|operand ? stack' ? H_operand_bool H_stack']; cbn.
     assert (exists b, operand = ValueImpl.Bool b) as [b H_operand_eq]. {
       destruct operand; cbn; try contradiction; sfirstorder.
     }
     rewrite H_operand_eq; clear H_operand_eq; cbn.
-    apply H_stack.
+    apply H_stack'.
   }
   { guard_instruction (Bytecode.Branch z).
     apply H_interpreter.
   }
   { guard_instruction (Bytecode.LdU8 z).
-    destruct_push.
+    destruct_abstract_push.
     lib.step; cbn; [|exact I].
     unfold IsInterpreterContextOfType.t; cbn.
     unfold IsStackValueOfType.t; cbn.
@@ -151,7 +165,7 @@ Proof.
     hauto l: on.
   }
   { guard_instruction (Bytecode.LdU64 z).
-    destruct_push.
+    destruct_abstract_push.
     lib.step; cbn; [|exact I].
     unfold IsInterpreterContextOfType.t; cbn.
     unfold IsStackValueOfType.t; cbn.
@@ -159,7 +173,7 @@ Proof.
     hauto l: on.
   }
   { guard_instruction (Bytecode.LdU128 z).
-    destruct_push.
+    destruct_abstract_push.
     lib.step; cbn; [|exact I].
     unfold IsInterpreterContextOfType.t; cbn.
     unfold IsStackValueOfType.t; cbn.
@@ -167,29 +181,56 @@ Proof.
     hauto l: on.
   }
   { guard_instruction Bytecode.CastU8.
-    unfold_state_monad.
-    pose proof (
-      AbstractStack.flatten_pop type_safety_checker.(TypeSafetyChecker.stack)
-    ) as H_pop.
-    destruct AbstractStack.pop as [[[operand_ty |] stack_ty] |]; cbn; [|exact I | exact I].
+    destruct_abstract_pop H_interpreter.
     lib.step; cbn; [exact I|].
-    destruct_push.
-    admit.
+    destruct_abstract_push.
+    destruct stack as [|operand stack]; cbn; [exact I|].
+    destruct operand; cbn; try exact I; (
+      repeat (lib.step; cbn; [|exact I]);
+      unfold IsInterpreterContextOfType.t, IsStackValueOfType.t; cbn;
+      sauto lq: on
+    ).
   }
   { guard_instruction Bytecode.CastU64.
-    admit.
+    destruct_abstract_pop H_interpreter.
+    lib.step; cbn; [exact I|].
+    destruct_abstract_push.
+    destruct stack as [|operand stack]; cbn; [exact I|].
+    destruct operand; cbn; try exact I; (
+      repeat (lib.step; cbn; [|exact I]);
+      unfold IsInterpreterContextOfType.t, IsStackValueOfType.t; cbn;
+      sauto lq: on
+    ).
   }
   { guard_instruction Bytecode.CastU128.
-    admit.
+    destruct_abstract_pop H_interpreter.
+    lib.step; cbn; [exact I|].
+    destruct_abstract_push.
+    destruct stack as [|operand stack]; cbn; [exact I|].
+    destruct operand; cbn; try exact I; (
+      repeat (lib.step; cbn; [|exact I]);
+      unfold IsInterpreterContextOfType.t, IsStackValueOfType.t; cbn;
+      sauto lq: on
+    ).
   }
   { guard_instruction (Bytecode.LdConst t).
     admit.
   }
   { guard_instruction Bytecode.LdTrue.
-    admit.
+    destruct_abstract_push.
+    lib.step; cbn; [|exact I].
+    unfold IsInterpreterContextOfType.t; cbn.
+    unfold IsStackValueOfType.t; cbn.
+    rewrite H_push.
+    hauto l: on.
   }
   { guard_instruction Bytecode.LdFalse.
-    admit.
+    destruct_abstract_push.
+    lib.step; cbn; [|exact I].
+    unfold IsInterpreterContextOfType.t; cbn.
+    unfold IsStackValueOfType.t; cbn.
+    rewrite H_push.
+    hauto l: on.
   }
   { guard_instruction (Bytecode.CopyLoc z).
     admit.
@@ -231,6 +272,157 @@ Proof.
     admit.
   }
   { guard_instruction (Bytecode.ImmBorrowLoc z).
+    admit.
+  }
+  { guard_instruction (Bytecode.MutBorrowField t).
+    admit.
+  }
+  { guard_instruction (Bytecode.MutBorrowFieldGeneric t).
+    admit.
+  }
+  { guard_instruction (Bytecode.ImmBorrowField t).
+    admit.
+  }
+  { guard_instruction (Bytecode.ImmBorrowFieldGeneric t).
+    admit.
+  }
+  { guard_instruction (Bytecode.MutBorrowGlobalDeprecated t).
+    admit.
+  }
+  { guard_instruction (Bytecode.MutBorrowGlobalGenericDeprecated t).
+    admit.
+  }
+  { guard_instruction (Bytecode.ImmBorrowGlobalDeprecated t).
+    admit.
+  }
+  { guard_instruction (Bytecode.ImmBorrowGlobalGenericDeprecated t).
+    admit.
+  }
+  { guard_instruction Bytecode.Add.
+    do 2 destruct_abstract_pop H_interpreter.
+    lib.step; cbn; [|exact I].
+    destruct_abstract_push.
+    destruct stack as [|operand1 stack]; cbn; [exact I|].
+    admit.
+  }
+  { guard_instruction Bytecode.Sub.
+    admit.
+  }
+  { guard_instruction Bytecode.Mul.
+    admit.
+  }
+  { guard_instruction Bytecode.Mod.
+    admit.
+  }
+  { guard_instruction Bytecode.Div.
+    admit.
+  }
+  { guard_instruction Bytecode.BitOr.
+    admit.
+  }
+  { guard_instruction Bytecode.BitAnd.
+    admit.
+  }
+  { guard_instruction Bytecode.Xor.
+    admit.
+  }
+  { guard_instruction Bytecode.Or.
+    admit.
+  }
+  { guard_instruction Bytecode.And.
+    admit.
+  }
+  { guard_instruction Bytecode.Not.
+    admit.
+  }
+  { guard_instruction Bytecode.Eq.
+    admit.
+  }
+  { guard_instruction Bytecode.Neq.
+    admit.
+  }
+  { guard_instruction Bytecode.Lt.
+    admit.
+  }
+  { guard_instruction Bytecode.Gt.
+    admit.
+  }
+  { guard_instruction Bytecode.Le.
+    admit.
+  }
+  { guard_instruction Bytecode.Ge.
+    admit.
+  }
+  { guard_instruction Bytecode.Abort.
+    admit.
+  }
+  { guard_instruction Bytecode.Nop.
+    admit.
+  }
+  { guard_instruction (Bytecode.ExistsDeprecated t).
+    admit.
+  }
+  { guard_instruction (Bytecode.ExistsGenericDeprecated t).
+    admit.
+  }
+  { guard_instruction (Bytecode.MoveFromDeprecated t).
+    admit.
+  }
+  { guard_instruction (Bytecode.MoveFromGenericDeprecated t).
+    admit.
+  }
+  { guard_instruction (Bytecode.MoveToDeprecated t).
+    admit.
+  }
+  { guard_instruction (Bytecode.MoveToGenericDeprecated t).
+    admit.
+  }
+  { guard_instruction Bytecode.Shl.
+    admit.
+  }
+  { guard_instruction Bytecode.Shr.
+    admit.
+  }
+  { guard_instruction (Bytecode.VecPack t z).
+    admit.
+  }
+  { guard_instruction (Bytecode.VecLen t).
+    admit.
+  }
+  { guard_instruction (Bytecode.VecImmBorrow t).
+    admit.
+  }
+  { guard_instruction (Bytecode.VecMutBorrow t).
+    admit.
+  }
+  { guard_instruction (Bytecode.VecPushBack t).
+    admit.
+  }
+  { guard_instruction (Bytecode.VecPopBack t).
+    admit.
+  }
+  { guard_instruction (Bytecode.VecUnpack t z).
+    admit.
+  }
+  { guard_instruction (Bytecode.VecSwap t).
+    admit.
+  }
+  { guard_instruction (Bytecode.LdU16 z).
+    admit.
+  }
+  { guard_instruction (Bytecode.LdU32 z).
+    admit.
+  }
+  { guard_instruction (Bytecode.LdU256 z).
+    admit.
+  }
+  { guard_instruction Bytecode.CastU16.
+    admit.
+  }
+  { guard_instruction Bytecode.CastU32.
+    admit.
+  }
+  { guard_instruction Bytecode.CastU256.
     admit.
   }
 Admitted.
